Inductive method for IL/F.

theories/Equiv/SimF.v
@@ -1,43 +1,167 @@
 Require Import List paco2.
-Require Export Util Var Val Exp Env Map CSet AutoIndTac IL AllInRel Sawtooth.
-Require Export Sim SimTactics IL InRel.
+Require Export Util Var Val Exp Env Map CSet AutoIndTac IL AllInRel.
+Require Export Sim SimTactics IL BlockType.
 
 Set Implicit Arguments.
 Unset Printing Records.
 
 (* A proof relation is parameterized by analysis information A *)
-Class ProofRelation (A:Type) := {
+Class ProofRelationF (A:Type) := {
     (* Relates parameter lists according to analysis information *)
-    ParamRel : A -> list var -> list var -> Prop;
+    ParamRelF : A -> list var -> list var -> Prop;
     (* Relates argument lists according to analysis information
        and closure environments *)
-    ArgRel : A -> list val -> list val -> Prop;
-    (* Relates blocks according to analysis information *)
-    IndexRel : 〔A〕 -> nat -> nat -> Prop;
+    ArgRelF : A -> list val -> list val -> Prop;
+    (* Relates environments according to analysis information *)
+    IndexRelF : 〔A〕 -> nat -> nat -> Prop;
     Image : 〔A〕 -> nat;
-    ArgLengthMatchI : forall a Z Z' VL VL',
-        ParamRel a Z Z' -> ArgRel a VL VL' -> length Z = length VL /\ length Z' = length VL';
-    IndexRelDrop : forall AL' AL n n', IndexRel (AL' ++ AL) n n' ->
+    IndexRelDrop : forall AL' AL n n', IndexRelF (AL' ++ AL) n n' ->
                                   n >= length AL'
-                                  -> IndexRel AL (n - length AL') (n' - Image AL')
-(*    IndexRelApp : forall AL AL' n n', IndexRelI AL n n' -> IndexRelI (AL' ++ AL) (❬AL'❭ + n) n' *)
+                                  -> IndexRelF AL (n - length AL') (n' - Image AL')
 }.
 
 Definition frel := rel3 simtype (fun _ : simtype => F.state)
                        (fun (_ : simtype) (_ : F.state) => F.state).
 
-Definition indexwise_r t (r:frel) A (PR:ProofRelation A) AL' E E' F F' AL L L' :=
+Coercion labN : lab >-> nat.
+
+Definition paramrel A (PR:ProofRelationF A) AL L L' :=
+  forall (f f':lab) E Z s i E' Z' s' i' a,
+    IndexRelF AL f f'
+    -> get AL f a
+    -> get L f (F.blockI E Z s i)
+    -> get L' f' (F.blockI E' Z' s' i')
+    -> ParamRelF a Z Z'.
+
+Definition app_r t (r:frel) A (PR:ProofRelationF A) AL L L' :=
+  forall (f f':lab) a E Z s i E' Z' s' i',
+    IndexRelF AL f f'
+    -> get AL f a
+    -> get L f (F.blockI E Z s i)
+    -> get L' f' (F.blockI E' Z' s' i')
+    -> forall E E' Yv Y'v Y Y',
+        ArgRelF a Yv Y'v
+        -> omap (op_eval E) Y = Some Yv
+        -> omap (op_eval E') Y' = Some Y'v
+        -> ❬Z❭ = ❬Yv❭
+        -> ❬Z'❭ = ❬Y'v❭
+        -> r t (L, E, stmtApp f Y)
+            (L', E', stmtApp f' Y').
+
+Lemma app_r_mon t (r r':frel) A (PR:ProofRelationF A) AL L L'
+  : app_r t r PR AL L L'
+    -> (forall t x y, r t x y -> r' t x y)
+    -> app_r t r' PR AL L L'.
+Proof.
+  intros Lr LE; hnf; intros; eauto.
+Qed.
+
+Definition indexes_exists {A} (PR:ProofRelationF A) AL (L L' : F.labenv) :=
+  forall n n' a b, IndexRelF AL n n' -> get AL n a -> get L n b -> exists b', get L' n' b'.
+
+Definition labenv_sim t (r:frel)
+           {A} (PR:ProofRelationF A) (AL:list A) L L' :=
+  length AL = length L /\
+  smaller L' /\
+  smaller L /\
+  paramrel PR AL L L' /\
+  indexes_exists PR AL L L' /\
+  app_r t r PR AL L L'.
+
+Lemma labenv_sim_nil t r A PR
+  : @labenv_sim t r A PR nil nil nil.
+Proof.
+  do 5 (try split); hnf; intros; isabsurd.
+Qed.
+
+Hint Immediate labenv_sim_nil.
+
+Lemma labenv_sim_mon t (r r':frel) A (PR:ProofRelationF A) AL L L'
+  :  labenv_sim t r PR AL L L'
+    -> (forall t x y, r t x y -> r' t x y)
+    -> labenv_sim t r' PR AL L L'.
+Proof.
+  intros [LEN [STL [STL' [PAR [IE SIM]]]]] LE; hnf; do 5 (try split); eauto.
+  eapply app_r_mon; eauto.
+Qed.
+
+Definition bodies_r t (r:frel) A (PR:ProofRelationF A) AL (L1 L2 L L':F.labenv) :=
+  forall f f' E Z s i E' Z' s' i' a,
+    IndexRelF AL f f'
+    -> get L f (F.blockI E Z s i)
+    -> get L' f' (F.blockI E' Z' s' i')
+    -> get AL f a
+    -> forall VL VL',
+        ArgRelF a VL VL'
+        -> r t (drop (f - i) L1, E[Z <-- List.map Some VL], s)
+            (drop (f' - i') L2, E'[Z' <-- List.map Some VL'], s').
+
+Lemma bodies_r_mon t (r r':frel) A (PR:ProofRelationF A) AL L1 L2 L L'
+  : bodies_r t r PR AL L1 L2 L L'
+    -> (forall t x y, r t x y -> r' t x y)
+    -> bodies_r t r' PR AL L1 L2 L L'.
+Proof.
+  intros Idx LE; hnf; intros; eauto.
+Qed.
+
+
+Lemma bodies_r_app_r t A (PR:ProofRelationF A) AL L L' r
+  : bodies_r t r PR AL L L' L L'
+    -> app_r t (sim'r r) PR AL L L'.
+Proof.
+  intros SIM.
+  hnf; intros.
+  pone_step; simpl; eauto with len.
+Qed.
+
+Lemma fix_compatible_bodies t A (PR:ProofRelationF A) AL L L'
+  : (forall (r:frel) L1 L2, app_r t (sim'r r) PR AL L1 L2
+          -> bodies_r t (sim'r r) PR AL L1 L2 L L')
+    -> forall r, bodies_r t (sim'r r) PR AL L L' L L'.
+Proof.
+  intros ISIM r.
+  pcofix CIH;
+  change (bodies_r t (sim'r r) PR AL L L' L L');
+  change (bodies_r t r PR AL L L' L L') in CIH.
+  eapply ISIM.
+  eapply bodies_r_app_r; eauto.
+Qed.
+
+Lemma stepGoto_mapi L blk Y E E'' vl f F k
+      (Ldef:get L (counted f - ❬F❭) blk)
+      (len:length (F.block_Z blk) = length Y)
+      (def:omap (op_eval E) Y = Some vl) E'
+      (updOk:F.block_E blk [F.block_Z blk <-- List.map Some vl] = E')
+      (ST:smaller L) (GE: counted f >= ❬F❭) (EQ:k = counted f - ❬F❭ - block_n blk)
+  : F.step (mapi (F.mkBlock E'') F ++ L, E, stmtApp f Y) EvtTau
+           (drop k L,
+            E', F.block_s blk).
+Proof.
+  subst.
+  rewrite <- (mapi_length (F.mkBlock E'')).
+  assert (counted f - block_n blk >= ❬mapi (F.mkBlock E'') F❭). {
+    exploit (ST _ _ Ldef).
+    rewrite mapi_length. simpl in *. omega.
+  }
+  orewrite (counted f - ❬mapi (F.mkBlock E'') F❭ - block_n blk
+            =  (counted f - block_n blk) - ❬mapi (F.mkBlock E'') F❭).
+  rewrite <- (drop_app_gen _ (mapi (F.mkBlock E'') F)); eauto.
+  eapply F.StepGoto; eauto.
+  rewrite get_app_ge. rewrite mapi_length. eauto. omega.
+Qed.
+
+Definition indexwise_r t (r:frel) A (PR:ProofRelationF A) AL' E E' F F' AL L L' :=
   forall n n' Z s Z' s' a,
-    IndexRel (AL' ++ AL) n n'
+    IndexRelF (AL' ++ AL) n n'
     -> get F n (Z,s)
     -> get F' n' (Z',s')
     -> get AL' n a
     -> forall VL VL',
-        ArgRel a VL VL'
+        ArgRelF a VL VL'
         -> r t (mapi (F.mkBlock E) F ++ L, E[Z <-- List.map Some VL], s)
             (mapi (F.mkBlock E') F' ++ L', E'[Z' <-- List.map Some VL'], s').
 
-Lemma indexwise_r_mon t (r r':frel) A (PR:ProofRelation A) AL' E E' F F' AL L L'
+Lemma indexwise_r_mon t (r r':frel) A (PR:ProofRelationF A) AL' E E' F F' AL L L'
   : indexwise_r t r PR AL' E E' F F' AL L L'
     -> (forall t x y, r t x y -> r' t x y)
     -> indexwise_r t r' PR AL' E E' F F' AL L L'.
@@ -45,179 +169,262 @@ Proof.
   intros Idx LE; hnf; intros; eauto.
 Qed.
 
-Definition simLabenv t (r:frel)
-           {A} (PR:ProofRelation A) (AL:list A) L L' :=
-  (length AL = length L /\ sawtooth L' /\ sawtooth L) /\
-  forall f f' a V Z s n V' Z' s' n',
-    IndexRel AL (counted f) (counted f')
-    -> get AL (counted f) a
-    -> get L (counted f) (F.blockI V Z s n)
-    -> get L' (counted f') (F.blockI V' Z' s' n')
-    -> ParamRel a Z Z'
-      /\ (forall E E' Yv Y'v Y Y',
-            ArgRel a Yv Y'v
-            -> omap (op_eval E) Y = Some Yv
-            -> omap (op_eval E') Y' = Some Y'v
-            -> sim'r r t (L, E, stmtApp f Y)
-                    (L', E', stmtApp f' Y')).
-
-Lemma simLabenv_mon t (r r':frel) A (PR:ProofRelation A) AL L L'
-  : simLabenv t r PR AL L L'
-    -> (forall t x y, r t x y -> r' t x y)
-    -> simLabenv t r' PR AL L L'.
-Proof.
-  intros [[? ?] SIM] LE; hnf; intros; split; eauto.
-  intros. edestruct SIM as [? SIM']; eauto.
-  split; eauto. intros.
-  eapply paco3_mon. eapply SIM; eauto. eauto.
-Qed.
-
-Definition indexwise_proofrel A (PR:ProofRelation A) (F F':〔params * stmt〕) AL' AL :=
+Definition indexwise_paramrel A (PR:ProofRelationF A) (F F':〔params * stmt〕) AL' AL :=
   forall n n' Z s Z' s' a,
-    IndexRel (AL' ++ AL) n n'
+    IndexRelF (AL' ++ AL) n n'
     -> get F n (Z,s)
     -> get F' n' (Z',s')
     -> get AL' n a
-    -> ParamRel a Z Z'.
+    -> ParamRelF a Z Z'.
 
+Definition separates A (PR:ProofRelationF A) AL' AL (F F':〔params * stmt〕) :=
+  length AL' = length F
+  /\ Image AL' = length F'
+  /\ (forall n n', IndexRelF (AL' ++ AL) n n' -> n < length F -> n' < length F')
+  /\  (forall n n', IndexRelF (AL' ++ AL) n n' -> n >= length F -> n' >= length F').
 
-Lemma stepGoto_mapi L blk Y E vl f F V
-      (Ldef:get L (counted f - ❬F❭) blk)
-      (len:length (F.block_Z blk) = length Y)
-      (def:omap (op_eval V) Y = Some vl) E'
-      (updOk:F.block_E blk [F.block_Z blk <-- List.map Some vl] = E')
-      (ST:sawtooth L) (GE: counted f >= ❬F❭)
-  : F.step (mapi (F.mkBlock E) F ++ L, V, stmtApp f Y) EvtTau
-           (drop (counted f - ❬F❭ - block_n blk) L,
-            E', F.block_s blk).
+Lemma complete_paramrel A (PR:ProofRelationF A) E E' F F' AL' AL L L'
+  : indexwise_paramrel PR F F' AL' AL
+    -> paramrel PR AL L L'
+    -> separates PR AL' AL F F'
+    -> paramrel PR (AL' ++ AL) (mapi (F.mkBlock E) F ++ L) (mapi (F.mkBlock E') F' ++ L').
 Proof.
-  rewrite <- (mapi_length (F.mkBlock E)).
-  assert (counted f - block_n blk >= ❬mapi (F.mkBlock E) F❭). {
-    exploit (sawtooth_smaller ST Ldef).
-    rewrite mapi_length. simpl in *. omega.
-  }
-  orewrite (counted f - ❬mapi (F.mkBlock E) F❭ - block_n blk
-            =  (counted f - block_n blk) - ❬mapi (F.mkBlock E) F❭).
-  rewrite <- (drop_app_gen _ (mapi (F.mkBlock E) F)); eauto.
-  eapply F.StepGoto; eauto.
-  rewrite get_app_ge. rewrite mapi_length. eauto. omega.
+  intros IPR PAR [Len1 [Img [Ilt Ige]]].
+  hnf; intros ? ? ? ? ? ? ? ? ? ? ? RN GetAL GetFL GetL'.
+  eapply get_app_cases in GetFL; destruct GetFL as [GetFL'| [GetFL GE]].
+  - exploit Ilt; eauto. eapply get_range in GetFL'.
+    rewrite mapi_length in GetFL'; eauto.
+    eapply get_app_lt_1 in GetL'; [| rewrite mapi_length; eauto ].
+    inv_get. destruct x0 as [Z s], x as [Z' s']. simpl in *. clear EQ0 EQ.
+    eauto.
+  - rewrite mapi_length in *; eauto.
+    exploit Ige; eauto.
+    eapply get_app_right_ge in GetAL; [ | rewrite Len1; eauto ].
+    eapply get_app_right_ge in GetL'; [ | rewrite mapi_length; eauto ].
+    eapply IndexRelDrop in RN; [| rewrite Len1; rewrite mapi_length in *; eauto].
+    exploit (PAR (LabI  (f - ❬AL'❭)) (LabI (f' - Image AL'))); eauto.
+    rewrite Len1; eauto. rewrite Img; rewrite mapi_length in *; eauto.
 Qed.
 
-Lemma simLabenv_extension' t (r:frel) A (PR:ProofRelation A) (AL AL':list A) E E' F F' L L'
-      (LEN1:length AL' = length F)
-  : indexwise_r t (sim'r r \3/ r) PR AL' E E' F F' AL L L'
-    -> indexwise_proofrel PR F F' AL' AL
-    -> (forall n n', IndexRel (AL' ++ AL) n n' -> n < length F -> n' < length F')
-    -> (forall n n', IndexRel (AL' ++ AL) n n' -> n >= length F -> n' >= length F')
-    -> Image AL' = length F'
-    -> simLabenv t r PR AL L L'
-    -> simLabenv t r PR (AL' ++ AL)
-                (mapi (F.mkBlock E) F ++ L)
-                (mapi (F.mkBlock E') F' ++ L').
+Lemma complete_indexes_exists A (PR:ProofRelationF A) E E' F F' AL' AL L L'
+  : indexes_exists PR AL L L'
+    -> separates PR AL' AL F F'
+    -> indexes_exists PR (AL' ++ AL) (mapi (F.mkBlock E) F ++ L) (mapi (F.mkBlock E') F' ++ L').
 Proof.
-  intros ISIM IP Ilt Ige Img SIML.
-  hnf. split.
-  destruct SIML; dcr; split; eauto with len. split; eauto.
-  econstructor; eauto. eapply tooth_F_mkBlocks.
-  econstructor; eauto. eapply tooth_F_mkBlocks.
+  intros IE [Len1 [Img [Ilt Ige]]].
+  hnf; intros ? ? ? ? RN GetAL GetF.
+  assert (Len3:forall E, ❬AL'❭ = ❬mapi (F.mkBlock E) F❭) by eauto with len.
+  eapply get_app_cases in GetF. destruct GetF as [GetF| [GetFL GE]].
+  + inv_get. exploit Ilt; eauto using get_range.
+    edestruct get_in_range; eauto.
+    eexists; eapply get_app, get_mapi; eauto.
+  + eapply get_app_right_ge in GetAL; [ | erewrite Len3; eauto ].
+    exploit Ige; eauto. rewrite mapi_length in *; eauto.
+    eapply IndexRelDrop in RN; [| erewrite Len3; eauto].
+    edestruct IE; eauto. erewrite Len3. eauto.
+    rewrite Img in H0. eexists.
+    eapply get_app_right; eauto. rewrite mapi_length in *. omega.
+Qed.
+
+Hint Unfold separates.
+
+Lemma labenv_sim_extension' t r A (PR:ProofRelationF A) (AL AL':list A) E E' F F' L L'
+  : indexwise_r t (sim'r r \3/ r) PR AL' E E' F F' AL L L'
+    -> indexwise_paramrel PR F F' AL' AL
+    -> separates PR AL' AL F F'
+    -> labenv_sim t (sim'r r) PR AL L L'
+    -> labenv_sim t (sim'r r) PR (AL' ++ AL) (mapi (F.mkBlock E) F ++ L) (mapi (F.mkBlock E') F' ++ L').
+Proof.
+  intros SIM IPR [Len2 [Img [Ilt Ige]]] [Len1 [STL [STL' [PAR [IE LSIM]]]]].
+  hnf; do 5 (try split);
+    eauto 20 using smaller_F_mkBlocks, complete_paramrel, complete_indexes_exists with len.
   intros f f' ? ? ? ? ? ? ? ? ? RN GetAL GetFL GetL'.
-  assert (❬AL'❭ = ❬mapi (F.mkBlock E) F❭) by eauto with len.
-  eapply get_app_cases in GetAL. destruct GetAL as [GetAL'|GetAL].
-  - eapply get_app_lt_1 in GetFL; [| rewrite <- H; eauto using get_range].
-    inv_get. destruct x as [Z s]. simpl in *. clear EQ.
-    exploit Ilt; eauto using get_range.
-    eapply get_app_lt_1 in GetL'; [| rewrite mapi_length; eauto with len ].
-    inv_get. destruct x as [Z' s']; simpl in *; clear EQ.
-    split; eauto.
-    intros.
-    exploit (ArgLengthMatchI); eauto; dcr.
-    pone_step; eauto using get_app, get_mapi; eauto; simpl; eauto with len.
-    orewrite (labN f - labN f = 0); simpl.
-    orewrite (labN f' - labN f' = 0); simpl.
-    eapply ISIM; eauto.
-  - destruct SIML; dcr.
-    eapply get_app_right_ge in GetFL; [ | rewrite <- H; eauto].
-    exploit Ige; eauto; try congruence.
-    eapply get_app_right_ge in GetL'; [ | eauto with len; rewrite mapi_length; eauto].    rewrite mapi_length in *.
-    eapply IndexRelDrop in RN; eauto.
-    edestruct (H1 (LabI (counted f - ❬AL'❭)) (LabI (counted f' - Image AL')))
-      as [? SIM]; simpl; eauto.
-    rewrite H; eauto. rewrite Img; eauto.
-    split; eauto.
-    intros.
-    exploit (ArgLengthMatchI); eauto; dcr.
+  assert (Len3:forall E, ❬AL'❭ = ❬mapi (F.mkBlock E) F❭) by eauto with len.
+  eapply get_app_cases in GetFL. destruct GetFL as [GetFL'| [GetFL GE]].
+  - exploit Ilt; eauto. eapply get_range in GetFL'.
+    rewrite mapi_length in GetFL'; eauto.
+    eapply get_app_lt_1 in GetL'; [| rewrite mapi_length; eauto ].
+    inv_get. destruct x0 as [Z s], x as [Z' s']. simpl in *. clear EQ0 EQ.
+    pone_step; simpl; eauto using get_app, get_mapi; simpl; eauto with len.
+    orewrite (f-f=0). orewrite (f'-f'=0). simpl.
+    exploit SIM; eauto.
+  - exploit Ige; eauto. rewrite mapi_length in GE; eauto.
+    eapply get_app_right_ge in GetAL; [ | rewrite (Len3 E); eauto ].
+    eapply get_app_right_ge in GetL'; [ | rewrite mapi_length; eauto ].
+    rewrite mapi_length in *.
+    eapply IndexRelDrop in RN; eauto; [| rewrite (Len3 E); eauto].
+    exploit (LSIM (LabI  (f - ❬AL'❭)) (LabI (f' - Image AL'))) as SIMR; eauto.
+    rewrite Len2; eauto. rewrite Img; eauto.
     eapply (@sim_Y_left F.state _ F.state _).
     eapply (@sim_Y_right F.state _ F.state _).
-    rewrite Img in SIM. rewrite H in SIM.
-    eapply SIM; eauto.
+    rewrite Img in SIMR. rewrite Len2 in SIMR.
+    eapply paco3_mon; [| eauto].
+    eapply SIMR; eauto.
     econstructor; simpl; eauto with len. simpl. eauto with len.
-    Focus 2.
+    eapply stepGoto_mapi; simpl in *; eauto with len.
     econstructor; simpl; eauto. simpl. eauto with len.
-    simpl.
-    eapply (stepGoto_mapi _ _ _ _ _ GetL'); simpl; eauto with len.
-    eapply (stepGoto_mapi _ _ _ _ _ GetFL); simpl; eauto with len.
-    simpl in *; omega.
+    eapply stepGoto_mapi; simpl in *; eauto with len.
+    erewrite <- Len3, Len2; eauto.
 Qed.
 
-Lemma fix_compatible_I t A (PR:ProofRelation A) AL F F' E E' L L' AL'
-(LEN2:length AL' = length F)
-  : (forall r, simLabenv t r PR (AL' ++ AL) (mapi (F.mkBlock E) F ++ L)
-                     (mapi (F.mkBlock E') F' ++ L')
-            -> indexwise_r t (sim'r r) PR AL' E E' F F' AL L L')
-    -> indexwise_proofrel PR F F' AL' AL
-    -> (forall n n', IndexRel (AL' ++ AL) n n' -> n < length F -> n' < length F')
-    -> (forall n n', IndexRel (AL' ++ AL) n n' -> n >= length F -> n' >= length F')
-    -> Image AL' = length F'
-    -> forall r, simLabenv t r PR AL L L'
+Lemma fix_compatible_separate t A (PR:ProofRelationF A) AL' AL E E' F F' L L'
+  : (forall r,
+        labenv_sim t (sim'r r) PR (AL' ++ AL) (mapi (F.mkBlock E) F ++ L) (mapi (F.mkBlock E') F' ++ L')
+        -> indexwise_r t (sim'r r) PR AL' E E' F F' AL L L')
+    -> indexwise_paramrel PR F F' AL' AL
+    -> separates PR AL' AL F F'
+    -> forall r, labenv_sim t (sim'r r) PR AL L L'
            -> indexwise_r t (sim'r r) PR AL' E E' F F' AL L L'.
 Proof.
-  intros ISIM IP Ilt Ige Img r SIML; pcofix CIH.
-  eapply ISIM; eauto.
-  hnf. split.
-  destruct SIML; dcr; split; eauto with len. split.
-  econstructor; eauto. eapply tooth_F_mkBlocks.
-  econstructor; eauto. eapply tooth_F_mkBlocks.
-  eapply simLabenv_extension'; eauto using simLabenv_mon, indexwise_r_mon.
+  intros ISIM LP SEP r SIML. pcofix CIH.
+  eapply ISIM.
+  eapply labenv_sim_extension'; eauto.
+  eauto using indexwise_r_mon; eauto.
+  eapply labenv_sim_mon; eauto.
+  intros. eapply paco3_mon; eauto.
 Qed.
 
-Lemma simILabenv_extension t A (PR:ProofRelation A) (AL AL':list A) E E' F F' L L'
-      (LEN1:length AL' = length F)
-  : (forall r, simLabenv t r PR (AL' ++ AL) (mapi (F.mkBlock E) F ++ L)
-                     (mapi (F.mkBlock E') F' ++ L')
-          -> indexwise_r t (sim'r r) PR AL' E E' F F' AL L L')
-    -> indexwise_proofrel PR F F' AL' AL
-    -> (forall n n', IndexRel (AL' ++ AL) n n' -> n < length F -> n' < length F')
-    -> (forall n n', IndexRel (AL' ++ AL) n n' -> n >= length F -> n' >= length F')
-    -> Image AL' = length F'
-    -> forall r, simLabenv t r PR AL L L'
-           -> simLabenv t r PR (AL' ++ AL)
-                       (mapi (F.mkBlock E) F ++ L)
-                       (mapi (F.mkBlock E') F' ++ L').
+
+Lemma labenv_sim_extension t A (PR:ProofRelationF A) (AL AL':list A) E E' F F' L L'
+  : (forall r,
+        labenv_sim t (sim'r r) PR (AL' ++ AL) (mapi (F.mkBlock E) F ++ L) (mapi (F.mkBlock E') F' ++ L')
+        -> indexwise_r t (sim'r r) PR AL' E E' F F' AL L L')
+    -> indexwise_paramrel PR F F' AL' AL
+    -> separates PR AL' AL F F'
+    -> forall r, labenv_sim t (sim'r r) PR AL L L'
+           -> labenv_sim t (sim'r r) PR (AL' ++ AL) (mapi (F.mkBlock E) F ++ L) (mapi (F.mkBlock E') F' ++ L').
 Proof.
-  intros. eapply simLabenv_extension'; eauto.
+  intros ISIM IP SEP r SIML.
+  eapply labenv_sim_extension'; eauto.
   eapply indexwise_r_mon.
-  eapply fix_compatible_I; eauto. eauto.
+  eapply fix_compatible_separate; eauto. eauto.
 Qed.
 
-Lemma simLabenv_extension_len t A (PR:ProofRelation A) (AL AL':list A)
-      E E' F F' L L'
-      (LEN1:length AL' = length F) (LEN2:length F = length F')
-      (IDX:forall AL n n', IndexRel AL n n' = (n = n'))
-  : (forall r, simLabenv t r PR (AL' ++ AL) (mapi (F.mkBlock E) F ++ L)
-                     (mapi (F.mkBlock E') F' ++ L')
+Lemma sim_fun t A (PR:ProofRelationF A) (AL AL':list A) E E' F F' L L' s s'
+  : (forall r, labenv_sim t (sim'r r) PR (AL' ++ AL) (mapi (F.mkBlock E) F ++ L) (mapi (F.mkBlock E') F' ++ L')
+          -> (sim'r r \3/ r) t (mapi (F.mkBlock E) F ++ L, E, s) (mapi (F.mkBlock E') F' ++ L', E', s'))
+    -> (forall r,
+          labenv_sim t (sim'r r) PR (AL' ++ AL) (mapi (F.mkBlock E) F ++ L) (mapi (F.mkBlock E') F' ++ L')
           -> indexwise_r t (sim'r r) PR AL' E E' F F' AL L L')
-    -> indexwise_proofrel PR F F' AL' AL
-    -> Image AL' = length F'
-    -> forall r, simLabenv t r PR AL L L'
-           -> simLabenv t r PR (AL' ++ AL)
-                       (mapi (F.mkBlock E) F ++ L)
-                       (mapi (F.mkBlock E') F' ++ L').
+    -> indexwise_paramrel PR F F' AL' AL
+    -> separates PR AL' AL F F'
+    -> forall r, labenv_sim t (sim'r r) PR AL L L'
+           -> sim'r r t (L, E, stmtFun F s) (L', E', stmtFun F' s').
+
 Proof.
-  assert (forall n n', IndexRel (AL' ++ AL) n n' -> n < length F -> n' < length F').
-  intros. rewrite IDX in H. subst; omega.
-  assert (forall n n', IndexRel (AL' ++ AL) n n' -> n >= length F -> n' >= length F').
-  intros. rewrite IDX in H0. subst; omega.
-  intros. eapply simLabenv_extension'; eauto.
+  intros SIM_s ISIM IP SEP r SIML.
+  pone_step.
+  eapply SIM_s.
+  eapply labenv_sim_extension; eauto.
+Qed.
+
+
+(* A proof relation is parameterized by analysis information A *)
+Class PointwiseProofRelationF (A:Type) := {
+    (* Relates parameter lists according to analysis information *)
+    ParamRelFP : A -> list var -> list var -> Prop;
+    (* Relates argument lists according to analysis information
+       and closure environments *)
+    ArgRelFP :  A -> list val -> list val -> Prop;
+    (* Relates environments according to analysis information *)
+}.
+
+Lemma pointwise_PR_as_PR A
+  : PointwiseProofRelationF A -> ProofRelationF A.
+Proof.
+  intros. destruct X as [B C].
+  eapply (Build_ProofRelationF B C (fun L n n' => eq n n') (@length _)).
+  - intros; dcr; subst; eauto.
+Defined.
+
+Arguments pointwise_PR_as_PR : simpl never.
+
+Hint Resolve pointwise_PR_as_PR : typeclass_instances.
+Coercion pointwise_PR_as_PR : PointwiseProofRelationF >-> ProofRelationF.
+
+Lemma IndexRelFP_eq A PR L n n'
+  : @IndexRelF A (pointwise_PR_as_PR PR) L n n' <-> n = n'.
+Proof.
+  destruct PR; simpl. reflexivity.
+Qed.
+
+Lemma IndexRelFP_refl A PR L n
+  : @IndexRelF A (pointwise_PR_as_PR PR) L n n.
+Proof.
+  destruct PR; simpl. reflexivity.
+Qed.
+
+Hint Resolve IndexRelFP_refl.
+
+Lemma labenv_sim_extension_ptw t A (PR:PointwiseProofRelationF A) (AL AL':list A) E E' F F' L L'
+  : (forall r ,
+        labenv_sim t (sim'r r) PR (AL' ++ AL) (mapi (F.mkBlock E) F ++ L) (mapi (F.mkBlock E') F' ++ L')
+        -> indexwise_r t (sim'r r) PR AL' E E' F F' AL L L')
+    -> indexwise_paramrel PR F F' AL' AL
+    -> length AL' = length F
+    -> length F = length F'
+    -> forall r, labenv_sim t (sim'r r) PR AL L L'
+        -> labenv_sim t (sim'r r) PR (AL' ++ AL) (mapi (F.mkBlock E) F ++ L) (mapi (F.mkBlock E') F' ++ L').
+Proof.
+  intros ISIM IP Len1 Len2 r SIML.
+  assert (separates PR AL' AL F F'). {
+    destruct SIML; dcr.
+    hnf; destruct PR; simpl; repeat split; intros; omega.
+  }
+  eapply labenv_sim_extension'; eauto.
   eapply indexwise_r_mon.
-  eapply fix_compatible_I; eauto. eauto.
+  eapply fix_compatible_separate; eauto. eauto.
+Qed.
+
+Lemma sim_fun_ptw t A (PR:PointwiseProofRelationF A) (AL AL':list A) F F' L L' E E' s s'
+  : (forall r, labenv_sim t (sim'r r) PR (AL' ++ AL) (mapi (F.mkBlock E) F ++ L) (mapi (F.mkBlock E') F' ++ L')
+          -> (sim'r r \3/ r) t (mapi (F.mkBlock E) F ++ L, E, s) (mapi (F.mkBlock E') F' ++ L', E', s'))
+    -> (forall r,
+          labenv_sim t (sim'r r) PR (AL' ++ AL) (mapi (F.mkBlock E) F ++ L) (mapi (F.mkBlock E') F' ++ L')
+          -> indexwise_r t (sim'r r) PR AL' E E' F F' AL L L')
+    -> indexwise_paramrel PR F F' AL' AL
+    -> length AL' = length F
+    -> length F = length F'
+    -> forall r, labenv_sim t (sim'r r) PR AL L L'
+           -> sim'r r t (L, E, stmtFun F s) (L', E', stmtFun F' s').
+Proof.
+  intros SIM_s ISIM IP Len1 Len2 r SIML.
+  pone_step.
+  eapply SIM_s.
+  eapply labenv_sim_extension_ptw; eauto.
+Qed.
+
+Lemma labenv_sim_app i A (PR:ProofRelationF A) AL L L' r V V' Y Y' (f f':lab) a
+  : labenv_sim i (sim'r r) PR AL L L'
+    -> get AL f a
+    -> IndexRelF AL f f'
+    -> (forall E Z s n E' Z' s' n',
+         get L f (F.blockI E Z s n)
+         -> get L' f' (F.blockI E' Z' s' n')
+         -> ParamRelF a Z Z'
+         -> (forall Yv, omap (op_eval V) Y = ⎣ Yv ⎦ -> ❬Z❭ = ❬Yv❭
+                 -> exists Y'v, omap (op_eval V') Y' = ⎣ Y'v ⎦ /\
+                          ❬Z'❭ = ❬Y'v❭ /\ ArgRelF a Yv Y'v)
+           /\ (if isBisim i then
+                (omap (op_eval V) Y = None -> omap (op_eval V') Y' = None)
+                /\ (❬Z❭ <> ❬Y❭ -> ❬Z'❭ <> ❬Y'❭)
+              else True))
+    -> sim'r r i (L, V, stmtApp f Y) (L', V', stmtApp f' Y').
+Proof.
+  intros LSIM GetAL RN ALL.
+  edestruct LSIM as [Len1 [STL [STL' [PAR [IE SIM]]]]]; eauto; dcr.
+  inv_get. edestruct IE; eauto.
+  destruct x as [E Z s n], x0 as [E' Z' s' n'].
+  exploit PAR; eauto.
+  edestruct ALL as [A1 A2]; eauto; dcr.
+  case_eq (omap (op_eval V) Y); intros.
+  - decide (❬Z❭ = ❬Y❭).
+    + edestruct A1; dcr; eauto with len.
+    + destruct i; simpl in *; dcr.
+      * exploit H4; eauto.
+        pno_step.
+      * perr.
+  - destruct i; simpl in *; dcr.
+    + exploit H3; eauto. pno_step.
+    + perr.
 Qed.
